Coherence/DelocationAlgo.v
@@ -97,7 +97,7 @@ Fixpoint computeParameters (DL: list (set var)) (ZL:list (list var)) (AP:list (s
 
 Local Notation "≽" := (fstNoneOrR (flip Subset)).
 Local Notation "≼" := (fstNoneOrR (Subset)).
-Local Notation "A ≿ B" := (list_eq (fstNoneOrR (flip Subset)) A B) (at level 60).
+Local Notation "A ≿ B" := (PIR2 (fstNoneOrR (flip Subset)) A B) (at level 60).
 
 Instance fstNoneOrR_flip_Subset_trans {X} `{OrderedType X} : Transitive ≽.
 hnf; intros. inv H; inv H0.
@@ -111,22 +111,6 @@ hnf; intros. inv H; inv H0.
 - inv H1. econstructor. transitivity y0; eauto.
 Qed.
 
-Instance list_eq_trans {A} (R : relation A) `{Transitive _ R} :
-  Transitive (list_eq R).
-Proof.
-  intros; hnf; intros. general induction H0.
-  - inv H1. econstructor.
-  - inv H2. econstructor. eauto. eauto.
-Qed.
-
-Instance instance_list_eq_sym {A} (R : relation A) `{Symmetric _ R} :
-  Symmetric (list_eq R).
-Proof.
-  intros; hnf; intros. general induction H0.
-  - econstructor.
-  - econstructor; eauto.
-Qed.
-
 Lemma trs_monotone (DL DL' : list (option (set var))) ZL s lv a
  : trs DL ZL s lv a
    -> DL ≿ DL'
@@ -135,7 +119,7 @@ Proof.
   intros. general induction H; eauto 30 using trs, restrict_subset2, Subset_refl.
   + econstructor.
     eapply IHtrs; eauto. eapply restrict_subset2; eauto. reflexivity.
-  + destruct (list_eq_get H1 H); eauto; dcr. inv H4.
+  + destruct (PIR2_nth H1 H); eauto; dcr. inv H4.
     econstructor; eauto.
   + econstructor.
     eapply IHtrs; eauto.
@@ -147,6 +131,7 @@ Proof.
     eapply IHtrs2. constructor; eauto. reflexivity.
 Qed.
 
+(*
 Lemma list_eq_get2 {X:Type} (L L':list X) eqA n x
   : list_eq eqA L L' -> get L' n x -> exists x', get L n x' /\ eqA x' x.
 Proof.
@@ -155,15 +140,16 @@ Proof.
   inv H1. eauto using get.
   edestruct IHlist_eq; eauto. firstorder using get.
 Qed.
+*)
 
-Lemma list_eq_restrict A B s
+Lemma PIR2_restrict A B s
 :  A ≿ B
    -> restrict A s ≿ B.
 Proof.
   intros. general induction H; simpl.
   - econstructor.
   - econstructor; eauto.
-    + inv H; simpl.
+    + inv pf; simpl.
       * econstructor.
       * destruct if. econstructor; eauto. econstructor.
 Qed.
@@ -177,7 +163,7 @@ Qed.
 
 Lemma trs_monotone3 (DL : list (option (set var))) AP AP' ZL s lv a
  : trs DL (zip (fun Z a => match a with Some a => Z++to_list a | None => Z end) ZL AP) s lv a
-   -> list_eq (fstNoneOrR Subset) AP AP'
+   -> PIR2 (fstNoneOrR Subset) AP AP'
    -> trs DL (zip (fun Z a => match a with Some a => Z++to_list a | None => Z end) ZL AP') s lv a.
 Proof.
   intros. general induction H; eauto using trs.
@@ -185,7 +171,7 @@ Proof.
     eapply IHtrs; eauto. eapply list_eq_restrict; eauto.*)
   + edestruct get_zip as  [? []]; eauto; dcr.
 (*    destruct (list_eq_get2 H3 H7); eauto; dcr.*)
-    destruct (list_eq_get H1 H4); eauto; dcr.
+    destruct (PIR2_nth H1 H4); eauto; dcr.
     exploit zip_get. eapply H2. eapply H6.
     econstructor. eauto. eapply X.
   + econstructor; eauto.
@@ -213,11 +199,11 @@ Qed.
 
 Lemma trs_AP_seteq (DL : list (option (set var))) AP AP' s lv a
  : trs DL AP s lv a
-   -> list_eq elem_eq AP AP'
+   -> PIR2 elem_eq AP AP'
    -> trs DL AP' s lv a.
 Proof.
   intros. general induction H; eauto using trs.
-  + destruct (list_eq_get H1 H0); eauto; dcr.
+  + destruct (PIR2_nth H1 H0); eauto; dcr.
     econstructor; eauto.
   + econstructor.
     - eapply IHtrs1. econstructor; eauto; reflexivity.
@@ -227,11 +213,11 @@ Qed.
 
 Lemma trs_AP_incl (DL : list (option (set var))) AP AP' s lv a
  : trs DL AP s lv a
-   -> list_eq (fun x y => of_list y ⊆ of_list x) AP AP'
+   -> PIR2 (fun x y => of_list y ⊆ of_list x) AP AP'
    -> trs DL AP' s lv a.
 Proof.
   intros. general induction H; eauto using trs.
-  + destruct (list_eq_get H1 H0); eauto; dcr.
+  + destruct (PIR2_nth H1 H0); eauto; dcr.
     econstructor; eauto.
   + econstructor.
     - eapply IHtrs1. econstructor; eauto; reflexivity.
@@ -240,52 +226,45 @@ Qed.
 
 Lemma trs_AP_incl' (DL : list (option (set var))) AP AP' s lv a
  : trs DL AP s lv a
-   -> list_eq (fun x y => of_list x ⊆ of_list y) AP AP'
+   -> PIR2 (fun x y => of_list x ⊆ of_list y) AP AP'
    -> trs DL AP' s lv a.
 Proof.
   intros. general induction H; eauto using trs.
-  + destruct (list_eq_get H1 H0); eauto; dcr.
+  + destruct (PIR2_nth H1 H0); eauto; dcr.
     econstructor; eauto.
   + econstructor.
     - eapply IHtrs1. econstructor; eauto; reflexivity.
     - eapply IHtrs2. econstructor; eauto; reflexivity.
 Qed.
 
-Lemma list_eq_flip {X} (R:X->X->Prop) l l'
-      : list_eq R l l'
-        -> list_eq (flip R) l' l.
-Proof.
-  intros. general induction H.
-  - econstructor.
-  - econstructor; eauto.
-Qed.
 
-Definition map_to_list {X} `{OrderedType X} (AP:list (option (set X))) := List.map (fun a => match a with Some a => to_list a | None => nil end) AP.
+Definition map_to_list {X} `{OrderedType X} (AP:list (option (set X)))
+  := List.map (fun a => match a with Some a => to_list a | None => nil end) AP.
 
-Lemma list_eq_Subset_of_list (AP AP': list (option (set var)))
-: list_eq (fstNoneOrR Subset) AP AP'
-  -> list_eq (fun x y => of_list y ⊆ of_list x) (map_to_list AP') (map_to_list AP).
+Lemma PIR2_Subset_of_list (AP AP': list (option (set var)))
+: PIR2 (fstNoneOrR Subset) AP AP'
+  -> PIR2 (fun x y => of_list y ⊆ of_list x) (map_to_list AP') (map_to_list AP).
 Proof.
   intros. general induction H; simpl.
   + econstructor.
-  + econstructor. destruct a, a'; cset_tac; intuition.
-    - rewrite of_list_3. rewrite of_list_3 in H1. inv H. intuition.
-    - inv H.
+  + econstructor. destruct x, y; cset_tac; intuition.
+    - rewrite of_list_3 in *. rewrite of_list_3 in H0. inv pf; intuition.
+    - inv pf.
     - exfalso; cset_tac; intuition. simpl in *. cset_tac; intuition.
     - eauto.
 Qed.
 
 Lemma trs_monotone3' (DL : list (option (set var))) AP AP' s lv a
  : trs DL (List.map oto_list AP) s lv a
-   -> list_eq (fstNoneOrR Subset) AP AP'
+   -> PIR2 (fstNoneOrR Subset) AP AP'
    -> trs DL (List.map oto_list AP') s lv a.
 Proof.
-  intros. eapply trs_AP_incl'; eauto. eapply list_eq_flip.
-  eapply list_eq_Subset_of_list; eauto.
+  intros. eapply trs_AP_incl'; eauto. eapply PIR2_flip.
+  eapply PIR2_Subset_of_list; eauto.
 Qed.
 
 
-Lemma list_eq_addParam DL AP x
+Lemma PIR2_addParam DL AP x
   : length AP = length DL
     -> PIR2 Subset AP (addParam x DL AP).
 Proof.
@@ -300,10 +279,10 @@ Qed.
 
 
 
-Lemma list_eq_map_some {X} R (AP AP':list X)
+Lemma PIR2_map_some {X} R (AP AP':list X)
 : length AP = length AP'
-  -> list_eq R AP AP'
-  -> list_eq (fstNoneOrR R) (List.map Some AP) (List.map Some AP').
+  -> PIR2 R AP AP'
+  -> PIR2 (fstNoneOrR R) (List.map Some AP) (List.map Some AP').
 Proof.
   intros. general induction H0.
   + econstructor.
@@ -312,10 +291,10 @@ Proof.
     - eauto.
 Qed.
 
-Lemma list_eq_map_some_option {X} R (AP AP':list X)
+Lemma PIR2_map_some_option {X} R (AP AP':list X)
 : length AP = length AP'
-  -> list_eq R AP AP'
-  -> list_eq (option_eq R) (List.map Some AP) (List.map Some AP').
+  -> PIR2 R AP AP'
+  -> PIR2 (option_eq R) (List.map Some AP) (List.map Some AP').
 Proof.
   intros. general induction H0.
   + econstructor.
@@ -332,71 +311,71 @@ Proof.
   rewrite zip_length2; congruence.
 Qed.
 
-Lemma list_eq_ounion {X} `{OrderedType X} (A B C:list (option (set X)))
+Lemma PIR2_ounion {X} `{OrderedType X} (A B C:list (option (set X)))
 : length A = length B
   -> length B = length C
-  -> list_eq ≽ A C
-  -> list_eq ≽ B C
-  -> list_eq ≽ (zip ounion A B) C.
+  -> PIR2 ≽ A C
+  -> PIR2 ≽ B C
+  -> PIR2 ≽ (zip ounion A B) C.
 Proof.
   intros. eapply length_length_eq in H0. eapply length_length_eq in H1.
   general induction H0; inv H1; simpl.
   - econstructor.
   - simpl in *. inv H2; inv H3.
     exploit IHlength_eq; eauto.
-    inv H7; inv H8; simpl; try now (econstructor; [econstructor; eauto| eauto]).
+    inv pf; inv pf0; simpl; try now (econstructor; [econstructor; eauto| eauto]).
     econstructor; eauto. econstructor. unfold flip in *.
     cset_tac; intuition.
 Qed.
 
-Lemma list_eq_ounion' {X} `{OrderedType X} (A B C:list (option (set X)))
+Lemma PIR2_ounion' {X} `{OrderedType X} (A B C:list (option (set X)))
 : length A = length B
   -> length B = length C
-  -> list_eq ≼ C A
-  -> list_eq ≼ C B
-  -> list_eq ≼ C (zip ounion A B).
+  -> PIR2 ≼ C A
+  -> PIR2 ≼ C B
+  -> PIR2 ≼ C (zip ounion A B).
 Proof.
   intros. eapply length_length_eq in H0. eapply length_length_eq in H1.
   general induction H0; inv H1; simpl.
   - econstructor.
   - simpl in *. inv H2; inv H3.
     exploit IHlength_eq; eauto.
-    inv H7; inv H8; simpl; try now (econstructor; [econstructor; eauto| eauto]).
+    inv pf; inv pf0; simpl; try now (econstructor; [econstructor; eauto| eauto]).
     econstructor; eauto. econstructor. unfold flip in *.
     cset_tac; intuition.
 Qed.
 
-Lemma list_eq_ounion_AB {X} `{OrderedType X} (A A' B B':list (option (set X)))
+Lemma PIR2_ounion_AB {X} `{OrderedType X} (A A' B B':list (option (set X)))
 : length A = length A'
   -> length B = length B'
   -> length A = length B
-  -> list_eq ≼ A A'
-  -> list_eq ≼ B B'
-  -> list_eq ≼ (zip ounion A B) (zip ounion A' B').
+  -> PIR2 ≼ A A'
+  -> PIR2 ≼ B B'
+  -> PIR2 ≼ (zip ounion A B) (zip ounion A' B').
 Proof.
   intros. length_equify.
   general induction H0; inv H1; inv H2; simpl; econstructor.
   - inv H3; inv H4.
-    inv H8; inv H9; simpl; try econstructor.
+    inv pf; inv pf0; simpl; try econstructor.
     destruct y; simpl; eauto. econstructor. cset_tac; intuition.
     destruct y0; simpl; eauto. econstructor. cset_tac; intuition.
     cset_tac; intuition.
   - inv H3; inv H4. eapply IHlength_eq; eauto.
 Qed.
 
-Lemma list_eq_option_eq_Subset_zip {X} `{OrderedType X} (A B C:list (option (set X)))
+Lemma PIR2_option_eq_Subset_zip {X} `{OrderedType X} (A B C:list (option (set X)))
 : length A = length B
   -> length B = length C
-  -> list_eq (option_eq Subset) C A
-  -> list_eq (option_eq Subset) C B
-  -> list_eq (option_eq Subset) C (zip ounion A B).
+  -> PIR2 (option_eq Subset) C A
+  -> PIR2 (option_eq Subset) C B
+  -> PIR2 (option_eq Subset) C (zip ounion A B).
 Proof.
   intros. eapply length_length_eq in H0. eapply length_length_eq in H1.
   general induction H0; inv H1; simpl.
   - econstructor.
   - simpl in *. inv H2; inv H3.
     exploit IHlength_eq; eauto.
-    inv H7; inv H8; simpl; try now (econstructor; [econstructor; eauto| eauto]).
+    inv pf; inv pf0; simpl; try now (econstructor; [econstructor; eauto| eauto]).
     econstructor; eauto. econstructor. unfold flip in *.
     cset_tac; intuition.
 Qed.
@@ -427,7 +406,7 @@ Proof.
 Qed.
 
 Lemma computeParameters_length DL ZL AP s lv an' LV
-:live_sound Functional (zip pair DL ZL) s lv
+:live_sound FunctionalAndImperative (zip pair DL ZL) s lv
   -> computeParameters (zip lminus DL ZL) ZL AP s lv = (an', LV)
   -> length AP = length DL
   -> length DL = length ZL
@@ -511,7 +490,7 @@ Inductive ifSndR {X Y} (R:X -> Y -> Prop) : X -> option Y -> Prop :=
   | ifsndR_None x : ifSndR R x None
   | ifsndR_R x y : R x y -> ifSndR R x (Some y).
 
-Lemma list_eq_ifSndR_right {X} `{OrderedType X} A B C
+Lemma PIR2_ifSndR_right {X} `{OrderedType X} A B C
 : PIR2 (ifSndR Subset) B A
 -> PIR2 Subset C B
 -> PIR2 (ifSndR Subset) C A.
@@ -566,7 +545,7 @@ Qed.
 
 
 Lemma computeParameters_AP_LV DL ZL AP s lv an' LV
-:live_sound Functional (zip pair DL ZL) s lv
+:live_sound FunctionalAndImperative (zip pair DL ZL) s lv
   -> computeParameters (zip lminus DL ZL) ZL AP s lv = (an', LV)
   -> length AP = length DL
   -> length DL = length ZL
@@ -575,8 +554,8 @@ Proof.
   intros LS CPEQ LEQ.
   general induction LS; simpl in * |- *; repeat let_case_eq; invc CPEQ.
   - exploit IHLS; eauto using addParam_zip_lminus_length.
-    eapply list_eq_ifSndR_right. eapply X.
-    eapply list_eq_addParam; eauto.
+    eapply PIR2_ifSndR_right. eapply X.
+    eapply PIR2_addParam; eauto.
     rewrite zip_length2; eauto.
   - exploit IHLS1; eauto.
     exploit IHLS2; eauto.
@@ -591,8 +570,8 @@ Proof.
     general induction AP; simpl. econstructor.
     econstructor. econstructor. eauto.
   - exploit IHLS; eauto using addParam_zip_lminus_length.
-    eapply list_eq_ifSndR_right. eapply X.
-    eapply list_eq_addParam; eauto.
+    eapply PIR2_ifSndR_right. eapply X.
+    eapply PIR2_addParam; eauto.
     rewrite zip_length2; eauto.
   - exploit IHLS1. reflexivity. Focus 2. instantiate (6:=getAnn als::DL).
     instantiate (5:=Z::ZL). eapply eq. reflexivity. simpl.
@@ -604,7 +583,7 @@ Proof.
     eapply ifSndR_zip_ounion; eauto.
     eapply ifSndR_addAdds.
     rewrite zip_length2. eauto. eauto.
-    eapply list_eq_ifSndR_right; eauto.
+    eapply PIR2_ifSndR_right; eauto.
     eapply addParams_Subset. rewrite zip_length2; eauto.
 Qed.
 
@@ -662,7 +641,7 @@ Qed.
 
 
 Lemma computeParameters_LV_DL DL ZL AP s lv an' LV
-:live_sound Functional (zip pair DL ZL) s lv
+:live_sound FunctionalAndImperative (zip pair DL ZL) s lv
   -> computeParameters (zip lminus DL ZL) ZL AP s lv = (an', LV)
   -> length AP = length DL
   -> length DL = length ZL
@@ -711,17 +690,17 @@ Proof.
   - econstructor. cset_tac; intuition.
 Qed.
 
-Lemma zip_list_eq X Y (eqA:Y -> Y -> Prop) (f:X -> X -> Y) l l'
+Lemma zip_PIR2 X Y (eqA:Y -> Y -> Prop) (f:X -> X -> Y) l l'
   : (forall x y, eqA (f x y) (f y x))
-    -> list_eq eqA (zip f l l') (zip f l' l).
+    -> PIR2 eqA (zip f l l') (zip f l' l).
 Proof.
   general induction l; destruct l'; simpl; try now econstructor.
   econstructor; eauto.
 Qed.
 
-Lemma list_eq_zip_ounion {X} `{OrderedType X} (b:list (option (set X))) b'
+Lemma PIR2_zip_ounion {X} `{OrderedType X} (b:list (option (set X))) b'
   : length b = length b'
-    -> list_eq (fstNoneOrR Subset) b (zip ounion b b').
+    -> PIR2 (fstNoneOrR Subset) b (zip ounion b b').
 Proof.
   intros. eapply length_length_eq in H0.
   general induction H0; simpl.
@@ -730,9 +709,9 @@ Proof.
     + destruct x,y; simpl; econstructor; cset_tac; intuition.
 Qed.
 
-Lemma list_eq_zip_ounion' {X} `{OrderedType X} (b:list (option (set X))) b'
+Lemma PIR2_zip_ounion' {X} `{OrderedType X} (b:list (option (set X))) b'
   : length b = length b'
-    -> list_eq (fstNoneOrR Subset) b (zip ounion b' b).
+    -> PIR2 (fstNoneOrR Subset) b (zip ounion b' b).
 Proof.
   intros. eapply length_length_eq in H0.
   general induction H0; simpl.
@@ -764,7 +743,7 @@ Qed.
 Lemma zip_ominus_contra DL b b'
   : length DL = length b
     -> length b = length b'
-    -> list_eq (fstNoneOrR Subset) b b'
+    -> PIR2 (fstNoneOrR Subset) b b'
     -> zip ominus DL b ≿ zip ominus DL b'.
 Proof.
   intros. eapply length_length_eq in H. eapply length_length_eq in H0.
@@ -772,8 +751,8 @@ Proof.
   - reflexivity.
   - econstructor; eauto.
     + destruct y, y0; simpl; try now econstructor.
-      * inv H1. inv H5. econstructor. unfold flip; cset_tac; intuition.
-      * inv H1. inv H5.
+      * inv H1. inv pf. econstructor. unfold flip; cset_tac; intuition.
+      * inv H1. inv pf.
     + inv H1. eauto.
 Qed.
 
@@ -790,7 +769,7 @@ Proof.
   + cset_tac; intuition.
 Qed.
 
-Lemma list_eq_not_in LV x DL AP
+Lemma PIR2_not_in LV x DL AP
 : length DL = length AP
   -> PIR2 (ifSndR Subset) (addParam x DL AP) LV
   ->  forall (n : nat) (lv0 dl : set var),
@@ -915,9 +894,9 @@ Qed.
 Transparent addAdds.
 
 
-Lemma list_eq_addAdds s DL b
+Lemma PIR2_addAdds s DL b
 : length DL = length b
-  -> list_eq ≼ b (addAdds s DL b).
+  -> PIR2 ≼ b (addAdds s DL b).
 Proof.
   intros. eapply length_length_eq in H.
   general induction H.
@@ -934,7 +913,7 @@ Qed.
 Lemma computeParameters_trs DL ZL AP s an' LV lv
 : length DL = length ZL
   -> length ZL = length AP
-  -> live_sound Functional (zip pair DL ZL) s lv
+  -> live_sound FunctionalAndImperative (zip pair DL ZL) s lv
   -> computeParameters (zip lminus DL ZL) ZL AP s lv = (an', LV)
   -> PIR2 Subset AP (zip lminus DL ZL)
   -> trs (restrict (zip ominus (zip lminus DL ZL) LV) (getAnn lv))
@@ -956,7 +935,7 @@ Proof.
     assert (SEQ:lv ∩ (lv \ {{x}}) [=] lv \ {{x}}) by (cset_tac; intuition).
     rewrite SEQ. eapply restrict_zip_ominus; eauto.
     rewrite zip_length2; eauto.
-    eapply list_eq_not_in; try eapply X. rewrite zip_length2; congruence.
+    eapply PIR2_not_in; try eapply X. rewrite zip_length2; congruence.
   - repeat let_case_eq. invc H4.
     exploit computeParameters_length; eauto; try congruence. congruence.
     exploit computeParameters_length; try eapply eq; eauto; try congruence.
@@ -965,21 +944,21 @@ Proof.
     + eapply trs_monotone.
       eapply trs_monotone3'.
       eapply IHlive_sound1; try eapply eq; eauto; try congruence.
-      eapply list_eq_zip_ounion. congruence.
+      eapply PIR2_zip_ounion. congruence.
       eapply restrict_subset2; eauto.
       eapply zip_ominus_contra; try congruence.
       rewrite zip_length2; congruence.
       rewrite zip_length2; congruence.
-      eapply list_eq_zip_ounion; congruence.
+      eapply PIR2_zip_ounion; congruence.
     + eapply trs_monotone.
       eapply trs_monotone3'.
       eapply IHlive_sound2; try eapply eq0; eauto.
-      eapply list_eq_zip_ounion'. congruence.
+      eapply PIR2_zip_ounion'. congruence.
       eapply restrict_subset2; eauto.
       eapply zip_ominus_contra; eauto.
       rewrite zip_length2; congruence.
       rewrite zip_length2; congruence.
-      eapply list_eq_zip_ounion'; congruence.
+      eapply PIR2_zip_ounion'; congruence.
   - edestruct get_zip as [? [? []]]; dcr; eauto. inv H10.
     edestruct (get_length_eq _ H9 H4).
     exploit killExcept_get; eauto.
@@ -987,7 +966,8 @@ Proof.
     exploit (zip_get ominus). eapply X0. eapply X.
     exploit map_get_1. eapply X.
     econstructor.
-    eapply restrict_get. eapply X1. unfold lminus. cset_tac; intuition.
+    eapply restrict_get. eapply X1. unfold lminus.
+    simpl in *. cset_tac; intuition.
     eapply X2.
   - econstructor.
   - let_case_eq. inv H4.
@@ -1005,7 +985,7 @@ Proof.
     assert (SEQ:lv ∩ (lv \ {{x}}) [=] lv \ {{x}}) by (cset_tac; intuition).
     rewrite SEQ. eapply restrict_zip_ominus; eauto.
     rewrite zip_length2; eauto.
-    eapply list_eq_not_in; try eapply X. rewrite zip_length2; congruence.
+    eapply PIR2_not_in; try eapply X. rewrite zip_length2; congruence.
   - repeat let_case_eq. invc H4.
     exploit (computeParameters_length (getAnn als::DL) (Z::ZL)); try eapply eq0; simpl; eauto; try congruence.
     exploit (computeParameters_length (getAnn als::DL) (Z::ZL)); try eapply eq; simpl; eauto; try congruence.
@@ -1035,11 +1015,11 @@ Proof.
       clear_all; cset_tac; intuition.
       simpl in *.
       transitivity (zip ounion XL XL0).
-      eapply list_eq_zip_ounion; congruence.
-      eapply list_eq_ounion_AB; try congruence; try reflexivity.
+      eapply PIR2_zip_ounion; congruence.
+      eapply PIR2_ounion_AB; try congruence; try reflexivity.
       rewrite addAdds_length. rewrite zip_length2; congruence.
       rewrite zip_length2; congruence.
-      eapply list_eq_addAdds. repeat rewrite zip_length2; eauto; congruence.
+      eapply PIR2_addAdds. repeat rewrite zip_length2; eauto; congruence.
       eapply trs_monotone. simpl.
       simpl addAdds in X3.
       destruct (ounion x x0). simpl in *.
@@ -1103,11 +1083,11 @@ Proof.
       clear_all; cset_tac; intuition.
       simpl.       simpl in *.
       transitivity (zip ounion XL XL0).
-      eapply list_eq_zip_ounion'; eauto; congruence.
-      eapply list_eq_ounion_AB; try congruence; try reflexivity.
+      eapply PIR2_zip_ounion'; eauto; congruence.
+      eapply PIR2_ounion_AB; try congruence; try reflexivity.
       rewrite addAdds_length. rewrite zip_length2; congruence.
       rewrite zip_length2; congruence.
-      eapply list_eq_addAdds. repeat rewrite zip_length2; eauto; congruence.
+      eapply PIR2_addAdds. repeat rewrite zip_length2; eauto; congruence.
       eapply trs_monotone. simpl in X1.
       simpl. destruct (ounion x x0). simpl in *.
       eapply trs_AP_seteq. eapply X3.
@@ -1135,9 +1115,9 @@ Proof.
       simpl. simpl in *. eauto; congruence.
       repeat rewrite zip_length2; eauto.
       simpl. simpl in *. eauto; congruence.
-      eapply list_eq_trans. eapply fstNoneOrR_flip_Subset_trans2.
+      eapply PIR2_trans. eapply fstNoneOrR_flip_Subset_trans2.
       reflexivity. simpl.
-      eapply list_eq_zip_ounion'.
+      eapply PIR2_zip_ounion'.
       rewrite addAdds_length. rewrite zip_length2; eauto.
       rewrite zip_length2; eauto. symmetry; simpl in *; congruence.
 Qed.
@@ -1154,7 +1134,7 @@ Arguments oemp [X] {H} s.
 
 Lemma additionalParameters_live_monotone (LV':list (option (set var))) DL ZL s an' LV lv
 : length DL = length ZL
-  -> live_sound Functional (zip pair DL ZL) s lv
+  -> live_sound FunctionalAndImperative (zip pair DL ZL) s lv
   -> additionalParameters_live LV s lv an'
   -> PIR2 (ifFstR Subset) LV' (zip lminus DL ZL)
   -> additionalParameters_live (List.map (@oemp var _) LV') s lv an'.
@@ -1164,7 +1144,7 @@ Proof.
     edestruct PIR2_nth_2; eauto. eapply zip_get; eauto.
     dcr.
     econstructor.
-    eapply map_get_1; eauto. rewrite <- H9.
+    eapply map_get_1; eauto. simpl in *. rewrite <- H9.
     inv H12; simpl. cset_tac; intuition. eapply H5.
   - econstructor; eauto.
     exploit (IHadditionalParameters_live1 (Some (of_list Za)::LV') (getAnn ans_lv::DL) (Z::ZL0)); simpl; try congruence.
@@ -1179,7 +1159,7 @@ Qed.
 Lemma computeParameters_live DL ZL AP s an' LV lv
 : length DL = length ZL
   -> length ZL = length AP
-  -> live_sound Functional (zip pair DL ZL) s lv
+  -> live_sound FunctionalAndImperative (zip pair DL ZL) s lv
   -> computeParameters (zip lminus DL ZL) ZL AP s lv = (an', LV)
   -> PIR2 Subset AP (zip lminus DL ZL)
   -> additionalParameters_live (List.map (@oemp _ _) LV) s lv an'.
