RenameApart.v
@@ -1,243 +1,85 @@
 Require Import CSet Le.
 
 Require Import Plus Util Map.
-Require Import Env EnvTy IL Liveness Coherence Alpha Fresh Annotation.
+Require Import Env EnvTy IL Alpha Fresh Annotation RenamedApart SetOperations.
 
 Set Implicit Arguments.
-
-Lemma lookup_set_list_union X `{OrderedType X } ϱ Y s s'
-: lookup_set ϱ s[=]s' ->
-  lookup_set ϱ (fold_left union (List.map Exp.freeVars Y) s)
-             [=]  fold_left union (List.map (lookup_set ϱ) (List.map Exp.freeVars Y)) s'.
-Proof.
-  general induction Y; simpl; eauto.
-  eapply IHY; eauto. rewrite lookup_set_union; eauto.
-  rewrite H0. reflexivity. intuition.
-Qed.
-
-Instance fold_left_subset_morphism X `{OrderedType X}:
-  Proper (list_eq Subset ==> Subset ==> Subset) (fold_left union).
-Proof.
-  unfold Proper, respectful; intros.
-  general induction H0; simpl; eauto.
-  - rewrite IHlist_eq; eauto. reflexivity.
-    rewrite H0, H2. reflexivity.
-Qed.
 
 (** We first define [rename_apart' ϱ G s], a function that chooses
     a variable fresh for G at every binder, records the choice in ϱ,
     and renames all variables according to ϱ *)
 
-Fixpoint rename_apart' (ϱ:env var) (G:set var) (s:stmt) : set var * stmt:=
+Fixpoint renameApart' (ϱ:env var) (G:set var) (s:stmt) : set var * stmt:=
 match s with
    | stmtExp x e s0 =>
      let y := fresh G in
      let ϱ' := ϱ[x <- y] in
-     let (G', s') := rename_apart' ϱ' (G ∪ {{y}}) s0 in
-       (G', stmtExp y (rename_exp ϱ e) s')
+     let (G', s') := renameApart' ϱ' {y; G} s0 in
+       ({y; G'}, stmtExp y (rename_exp ϱ e) s')
    | stmtIf e s1 s2 =>
-     let (G', s1') := rename_apart' ϱ G s1 in
-     let (G'', s2') := rename_apart' ϱ G' s2 in
-      (G'', stmtIf (rename_exp ϱ e) s1' s2')
-   | stmtGoto l Y => (G, stmtGoto l (List.map (rename_exp ϱ) Y))
-   | stmtReturn e => (G, stmtReturn (rename_exp ϱ e))
+     let (G', s1') := renameApart' ϱ G s1 in
+     let (G'', s2') := renameApart' ϱ (G ∪ G') s2 in
+      (G' ∪ G'', stmtIf (rename_exp ϱ e) s1' s2')
+   | stmtGoto l Y => (∅, stmtGoto l (List.map (rename_exp ϱ) Y))
+   | stmtReturn e => (∅, stmtReturn (rename_exp ϱ e))
    | stmtExtern x f Y s =>
      let y := fresh G in
      let ϱ' := ϱ[x <- y] in
-     let (G', s') := rename_apart' ϱ' (G ∪ {{y}}) s in
-       (G', stmtExtern y f (List.map (rename_exp ϱ) Y) s')
+     let (G', s') := renameApart' ϱ' {y; G} s in
+       ({y; G'}, stmtExtern y f (List.map (rename_exp ϱ) Y) s')
    | stmtLet Z s1 s2 =>
      let Y := fresh_list fresh G (length Z) in
      let ϱZ := ϱ [ Z <-- Y ] in
-     let (G', s1') := rename_apart' ϱZ (G ∪ of_list Y) s1 in
-     let (G'', s2') := rename_apart' ϱ G' s2 in
-     (G'', stmtLet Y s1'  s2')
+     let (G', s1') := renameApart' ϱZ (G ∪ of_list Y) s1 in
+     let (G'', s2') := renameApart' ϱ (G ∪ (G' ∪ of_list Y)) s2 in
+     (G' ∪ (G'' ∪ of_list Y), stmtLet Y s1'  s2')
    end.
 
-Fixpoint rename_apart_rho (ϱ:env var) (s:stmt) : env var :=
-match s with
-   | stmtExp x e s0 =>
-     let y := fresh (freeVars s0 \ {{x}}) in
-     let ϱ' := ϱ[y <- x] in rename_apart_rho ϱ' s0
-   | stmtIf x s1 s2 =>
-     let ϱ' := rename_apart_rho ϱ s1 in rename_apart_rho ϱ' s2
-   | stmtGoto l Y => ϱ
-   | stmtReturn x => ϱ
-   | stmtExtern x f Y s =>
-     let y := fresh (freeVars s \ {{x}}) in
-     let ϱ' := ϱ[x <- y] in
-     rename_apart_rho ϱ' s
-   | stmtLet Z s1 s2 =>
-     let Y := fresh_list fresh (freeVars s1) (length Z) in
-     let ϱZ := ϱ [ Z <-- Y ]  in
-     let ϱ' := rename_apart_rho ϱZ s1 in rename_apart_rho ϱ' s2
-   end.
-
-
-Lemma rename_apart_incl ϱ G G' s
-  : G ⊆ G' -> G ⊆ fst (rename_apart' ϱ G' s).
+Lemma renameApart'_disj ϱ G s
+  : disj G (fst (renameApart' ϱ G s)).
 Proof.
   general induction s; simpl; repeat let_pair_case_eq; simpl; subst; eauto.
-  - eapply IHs. cset_tac. left; eauto.
-  - eapply IHs. cset_tac. left; eauto.
-  - eapply IHs2. eapply IHs1. cset_tac. left; eauto.
-Qed.
-
-Lemma rename_apart_incl_eq ϱ G G' s G''
-  : G ⊆ G' -> G'' = fst (rename_apart' ϱ G' s) -> G ⊆ G''.
-Proof.
-  intros; subst; eauto using rename_apart_incl.
-Qed.
-
-Lemma rename_apart_notOccur G G' ϱ s
-  : G ⊆ G'
-  -> lookup_set ϱ (freeVars s) ⊆ G'
-  -> notOccur (G \ lookup_set ϱ (freeVars s)) (snd (rename_apart' ϱ G' s)).
-Proof.
-  general induction s; simpl; repeat let_pair_case_eq; simpl; eauto using notOccur; subst; eauto.
-
-  - econstructor; simpl in *.
-    + intro. eapply fresh_spec. eapply H, minus_incl; eauto.
-    + eapply notOccur_incl. Focus 2. eapply IHs. eapply Subset_refl.
-      hnf; intros. eapply lookup_set_spec in H1. destruct H1; dcr.
-      lud. cset_tac; eauto. eapply union_2. eapply H0. eapply lookup_set_spec. intuition.
-      eexists x0; cset_tac; intuition. intuition.
-      hnf; intros. cset_tac. left; eauto. intro.
-      eapply H3. eapply lookup_set_spec. intuition.
-      eapply lookup_set_spec in H1. destruct H1; dcr; eauto. lud.
-      rewrite H5 in H2. exfalso. eapply fresh_spec; eauto.
-      exists x0. cset_tac; intuition. intuition.
-    + eapply notOccur_freeVars.
-      cset_tac; intuition. eapply rename_exp_freeVars in H3.
-      eapply H4. eapply lookup_set_incl; eauto; intuition. intuition.
-
-  - econstructor.
-    eapply Exp.notOccur_freeVars. cset_tac; intuition.
-    eapply rename_exp_freeVars in H3; eauto.
-    eapply H4. eapply lookup_set_spec; eauto. eapply lookup_set_spec in H3; eauto.
-    destruct H3. eexists x. cset_tac; intuition; eauto.
-
-    eapply notOccur_incl,IHs1.
-    eapply incl_minus_lr; eauto. eapply lookup_set_incl. intuition.
-    eapply union_incl_left, incl_left. reflexivity.
-
-    simpl in *; eauto. rewrite <- H0. eapply lookup_set_incl; eauto.
-    eapply union_incl_left, incl_left.
-
-    eapply notOccur_incl, IHs2.
-    eapply incl_minus_lr; eauto. eapply lookup_set_incl. intuition.
-    eapply union_incl_left, incl_right.
-    apply rename_apart_incl. reflexivity.
-    apply rename_apart_incl.
-    simpl in *. eapply Subset_trans; eauto. eapply lookup_set_incl; eauto.
+  - rewrite disj_add; split; eauto using fresh_spec.
+    eapply disj_subset_subset_flip_impl; [| reflexivity | eapply IHs].
     cset_tac; intuition.
-  - econstructor. intros.
-    edestruct map_get_4; eauto; dcr; subst.
-    eapply Exp.notOccur_freeVars. cset_tac; intuition.
-    eapply rename_exp_freeVars in H5; eauto.
-    eapply H6. eapply lookup_set_spec; eauto.
-    eapply lookup_set_spec in H5; eauto.
-    destruct H5; dcr. eexists x0; intuition.
-    eapply incl_list_union.
-    eapply map_get_1; eauto. reflexivity. eauto.
-  - econstructor.
-    eapply Exp.notOccur_freeVars. cset_tac; intuition.
-    eapply rename_exp_freeVars in H3; eauto.
-  - econstructor; eauto.
-    + intros.
-      edestruct map_get_4; eauto; dcr; subst.
-      eapply Exp.notOccur_freeVars. cset_tac; intuition.
-      eapply rename_exp_freeVars in H5; eauto.
-      eapply H6. eapply lookup_set_spec; eauto.
-      eapply lookup_set_spec in H5; eauto.
-      destruct H5; dcr. eexists x1; intuition.
-      eapply incl_right. eapply incl_list_union.
-      eapply map_get_1; eauto. reflexivity. eauto.
-    + intro. eapply fresh_spec. eapply H, minus_incl; eauto.
-    + eapply notOccur_incl.
-      Focus 2.
-      eapply IHs; try reflexivity.
-      hnf; intros. eapply lookup_set_spec in H1; eauto. destruct H1; dcr.
-      lud. cset_tac; eauto. eapply union_2. eapply H0.
-      eapply lookup_set_spec; eauto. intuition.
-      eexists x0; cset_tac; intuition. simpl.
-      eapply incl_left. cset_tac; intuition.
-      hnf; intros. cset_tac. left; eauto. intro.
-      eapply H3. eapply lookup_set_spec. intuition.
-      eapply lookup_set_spec in H1; eauto. destruct H1; dcr; eauto. lud.
-      rewrite H5 in H2. exfalso. eapply fresh_spec; eauto.
-      exists x0. cset_tac; intuition.
-  - econstructor.
-    + cset_tac; intuition. rewrite H in H1.
-      eapply (not_in_empty a). rewrite <- (fresh_set_spec fresh fresh_spec G' (length Z)).
-      cset_tac; eauto.
-    + eapply notOccur_incl. Focus 2. eapply IHs1. reflexivity.
-      rewrite lookup_set_update_with_list_in_union_length.
-      eapply incl_union_lr. simpl in *. eapply Subset_trans;try eassumption.
-      eapply lookup_set_incl. intuition.  cset_tac; eauto. reflexivity. intuition.
-      rewrite fresh_list_length; eauto.
-
-      hnf; intros. cset_tac. left; eauto. intro.
-      eapply lookup_set_spec in H1.
-      destruct H1; dcr. decide(x ∈ of_list Z).
-      eapply (update_with_list_lookup_in ϱ) with (Z':=fresh_list fresh G' (length Z)) in i; eauto.
-      rewrite <- H5 in i. apply (not_in_empty a).
-      eapply fresh_set_spec. eapply fresh_spec. cset_tac; eauto.
-      rewrite fresh_list_length; eauto.
-      eapply H3. eapply lookup_set_spec. intuition.
-      erewrite update_with_list_no_update in H5; eauto. eexists x.
-      split; eauto. cset_tac; eauto.
-      eapply update_with_list_proper.
-    + eapply notOccur_incl. Focus 2. eapply IHs2. reflexivity.
-      eapply Subset_trans. Focus 2. eapply rename_apart_incl. reflexivity.
-      eapply Subset_trans. Focus 2. eapply union_subset_1.
-      simpl in H0. rewrite <- H0. eapply lookup_set_incl. intuition. cset_tac.
-      intuition.
-      simpl in *. eapply Subset_trans. Focus 2. rewrite <- rename_apart_incl.
-      Focus 2. reflexivity. reflexivity.
-      eapply incl_minus_lr. cset_tac; intuition.
-      eapply lookup_set_incl; cset_tac; intuition.
+  - rewrite disj_app; split; eauto.
+    eapply disj_subset_subset_flip_impl; [| reflexivity | eapply IHs2].
+    cset_tac; intuition.
+  - rewrite disj_add; split; eauto using fresh_spec.
+    eapply disj_subset_subset_flip_impl; [| reflexivity | eapply IHs].
+    cset_tac; intuition.
+  - repeat (rewrite disj_app; split); eauto.
+    eapply disj_subset_subset_flip_impl; [| reflexivity | eapply IHs1].
+    cset_tac; intuition.
+    eapply disj_subset_subset_flip_impl; [| reflexivity | eapply IHs2].
+    cset_tac; intuition.
+    symmetry. eapply fresh_list_spec, fresh_spec.
 Qed.
 
-Opaque to_list.
-
-Fixpoint ssa_ann (s:stmt) (G:set var) : ann (set var * set var) :=
+Fixpoint renamedApartAnn (s:stmt) (G:set var) : ann (set var * set var) :=
   match s with
     | stmtExp x e s =>
-      let an := ssa_ann s (G ∪ {{x}}) in
-      ann1 (G,snd (getAnn an)) an
+      let an := renamedApartAnn s {x; G} in
+      ann1 (G, {x; snd (getAnn an) }) an
     | stmtIf e s t =>
-      let ans := ssa_ann s G in
-      let ant := ssa_ann t G in
+      let ans := renamedApartAnn s G in
+      let ant := renamedApartAnn t G in
       ann2 (G, snd (getAnn ans) ∪ snd (getAnn ant)) ans ant
     | stmtReturn e =>
-      ann0 (G, G)
+      ann0 (G, ∅)
     | stmtGoto f Y =>
-      ann0 (G, G)
+      ann0 (G, ∅)
     | stmtExtern x f Y s =>
-      let an := ssa_ann s (G ∪ {{x}}) in
-      ann1 (G,snd (getAnn an)) an
+      let an := renamedApartAnn s {x; G} in
+      ann1 (G, {x; snd (getAnn an)}) an
     | stmtLet Z s t =>
-      let ans := ssa_ann s (G ∪ of_list Z) in
-      let ant := ssa_ann t G in
-      ann2 (G, snd (getAnn ans) ∪ snd (getAnn ant)) ans ant
+      let ans := renamedApartAnn s (G ∪ of_list Z) in
+      let ant := renamedApartAnn t G in
+      ann2 (G, snd (getAnn ans) ∪ (snd (getAnn ant) ∪ of_list Z)) ans ant
   end.
 
-Instance pe_trans X `{OrderedType X} : Transitive (@pe _ _).
-Proof.
-  hnf; intros ? ? ? B C.
-  eapply prod_Equivalence_obligation_3; eauto using Equal_ST.
-Qed.
-
-Instance getAnn_ann_R_morphism A (R:A->A->Prop)
-: Proper (ann_R R ==> R) (getAnn).
-Proof.
-  unfold Proper, respectful; intros.
-  inv H; simpl; eauto.
-Qed.
-
-Instance ssa_ann_morph
-: Proper (eq ==> Equal ==> ann_R (@pe _ _ )) ssa_ann.
+Instance renamedApart_ann_morph
+: Proper (eq ==> Equal ==> ann_R (@pe _ _ )) renamedApartAnn.
 Proof.
   unfold Proper, respectful; intros. subst.
   general induction y; simpl; eauto using ann_R.
@@ -258,146 +100,38 @@ Proof.
     eapply IHy1. rewrite H0. reflexivity.
 Qed.
 
-Lemma ssa_ann_decomp s G
-: pe (getAnn (ssa_ann s G)) (G, snd (getAnn (ssa_ann s G))).
+Lemma fst_renamedApartAnn s G
+ : fst (getAnn (renamedApartAnn s G)) = G.
+Proof.
+  general induction s; eauto.
+Qed.
+
+
+Lemma snd_renameApartAnn s G ϱ G'
+: snd (getAnn (renamedApartAnn (snd (renameApart' ϱ G s)) G')) = fst (renameApart' ϱ G s).
+Proof.
+  general induction s; simpl; repeat let_pair_case_eq; simpl; eauto.
+  - subst. rewrite IHs. reflexivity.
+  - subst. rewrite IHs1. rewrite IHs2. reflexivity.
+  - subst. rewrite IHs. reflexivity.
+  - subst. rewrite IHs1. rewrite IHs2. reflexivity.
+Qed.
+
+Lemma renameApartAnn_decomp s G
+: pe (getAnn (renamedApartAnn s G)) (G, snd (getAnn (renamedApartAnn s G))).
 Proof.
   destruct s; simpl; try reflexivity.
-Qed.
-
-Lemma ssa_ann_app_incl s G G' G''
-: G' ∪ G'' [=] G
-  -> snd (getAnn (ssa_ann s G)) [=] G' ++ snd (getAnn (ssa_ann s G'')).
-Proof.
-  intros. general induction s; simpl.
-  - rewrite IHs. reflexivity. rewrite <- H. rewrite union_assoc. reflexivity.
-  - rewrite (IHs1 _ _ _ H) at 1.
-    erewrite (IHs2 _ _ {}); [|rewrite union_comm, empty_neutral_union; reflexivity].
-    symmetry.
-    erewrite (IHs2 _ _ {}); [|rewrite union_comm, empty_neutral_union; reflexivity].
-    (* rewrite (IHs1 _ _ _ H) at 1. *)
-    rewrite <- H.
-    clear_all; cset_tac; intuition.
-  - rewrite H. reflexivity.
-  - rewrite H. reflexivity.
-  - rewrite IHs. reflexivity. rewrite <- H. rewrite union_assoc. reflexivity.
-  - erewrite (IHs2 _ _ {}); [|rewrite union_comm, empty_neutral_union; reflexivity].
-    erewrite (IHs1 _ _ {}); [|rewrite union_comm, empty_neutral_union; reflexivity].
-    symmetry.
-    erewrite (IHs2 _ _ {}); [|rewrite union_comm, empty_neutral_union; reflexivity].
-    erewrite (IHs1 _ _ {}); [|rewrite union_comm, empty_neutral_union; reflexivity].
-    rewrite <- H. clear_all; cset_tac; intuition.
-Qed.
-
-Lemma rename_apart_fst_incl ϱ s G
-: G ⊆ fst (rename_apart' ϱ G s).
-Proof.
-  intros.
-  general induction s; simpl; repeat let_pair_case_eq; simpl; subst; eauto; try reflexivity; try now (rewrite <- IHs; cset_tac; intuition).
-  - rewrite <- IHs2, <- IHs1; reflexivity.
-  - rewrite <- IHs2, <- IHs1. cset_tac; intuition.
-Qed.
-
-Lemma rename_apart_fst_incl_app ϱ s G
-: fst (rename_apart' ϱ G s) [=] fst (rename_apart' ϱ G s) ∪ G.
-Proof.
-  pose proof (@rename_apart_fst_incl ϱ s G).
-  cset_tac; intuition.
-Qed.
-
-Lemma ssa_ann_rename_apart s G ϱ
-: snd (getAnn (ssa_ann (snd (rename_apart' ϱ G s)) G)) [=] fst (rename_apart' ϱ G s).
-Proof.
-  general induction s; simpl; repeat let_pair_case_eq; simpl; subst; eauto; try reflexivity.
-  - rewrite IHs1 at 1. rewrite <- IHs2. rewrite <- ssa_ann_app_incl. reflexivity.
-    rewrite rename_apart_fst_incl_app. cset_tac; intuition.
-  - rewrite <- IHs2. rewrite IHs1 at 1.
-    rewrite <- ssa_ann_app_incl. reflexivity.
-    symmetry.
-    rewrite rename_apart_fst_incl_app.
-    cset_tac; intuition.
-Qed.
-
-
-
-Lemma ssa_ann_rename_apart' s G G' ϱ
-: G ⊆ G'
-  -> snd (getAnn (ssa_ann (snd (rename_apart' ϱ G' s)) G)) [=] fst (rename_apart' ϱ G' s) \ (G' \ G).
-Proof.
-  general induction s; simpl; repeat let_pair_case_eq; simpl; subst; eauto; try reflexivity.
-  - rewrite IHs at 1. cset_tac; intuition.
-    eapply H0; intros. intuition.
-    eapply fresh_spec. instantiate (1:=G'). rewrite H2. eauto.
-    rewrite H. reflexivity.
-  - rewrite IHs1. rewrite IHs2.
-    rewrite rename_apart_fst_incl_app at 3.
-    cset_tac; intuition.
-    eapply rename_apart_fst_incl; eauto.
-    decide ( a \In fst (rename_apart' ϱ G' s1)); intuition.
-    rewrite H. eapply rename_apart_fst_incl; eauto. eauto.
-  - cset_tac; intuition. decide (a ∈ G); intuition.
-  - cset_tac; intuition. decide (a ∈ G); intuition.
-  - rewrite IHs; try reflexivity. cset_tac; intuition.
-    eapply H0; intros; intuition.
-    eapply fresh_spec. instantiate (1:=G'). rewrite H2. eauto.
-    rewrite H. reflexivity.
-  - rewrite IHs2. rewrite IHs1.
-    cset_tac; intuition.
-    + eapply rename_apart_fst_incl; eauto.
-    + eapply H1; intros. destruct H3; eauto; split; eauto.
-      exploit (fresh_list_spec fresh fresh_spec G' (length Z) a); dcr. cset_tac; intuition.
-    + eapply H1; intros.
-      eapply rename_apart_fst_incl; eauto. cset_tac; intuition. eauto.
-    + decide ( a \In
-                 fst
-                 (rename_apart' (ϱ [Z <-- fresh_list fresh G' (length Z)])
-                                (G' ++ of_list (fresh_list fresh G' (length Z))) s1)); intuition.
-    + rewrite H. reflexivity.
-    + rewrite <- rename_apart_fst_incl. rewrite H. eapply incl_left.
-Qed.
-
-Instance ann_R_trans A R `{Transitive A R} : Transitive (ann_R R).
-Proof.
-  hnf; intros ? ? ? B C.
-  general induction B; inv C; econstructor; eauto.
-Qed.
-
-Instance ann_R_ann1_pe_morphism X `{OrderedType X}
-: Proper (@pe X _ ==> ann_R (@pe X _) ==> ann_R (@pe X _)) (@ann1 _).
-Proof.
-  unfold Proper, respectful; intros.
-  econstructor; eauto.
-Qed.
-
-Instance pminus_morphism
-: Proper (Equal ==> (@pe _ _) ==> (@pe _ _) ) pminus.
-Proof.
-  unfold Proper, respectful; intros.
-  inv H0; simpl; econstructor. rewrite H1, <- H. reflexivity.
-  rewrite H2, H. reflexivity.
-Qed.
-
-Instance mapAnn_pminus_morphism G'
-  : Proper (ann_R (@pe _ _) ==> ann_R (@pe _ _)) (mapAnn (pminus G')).
-Proof.
-  unfold Proper, respectful; intros.
-  general induction H; simpl.
-  - econstructor; eauto.
-    + rewrite H. reflexivity.
-  - econstructor; eauto.
-    + rewrite H. reflexivity.
-  - econstructor; eauto.
-    + rewrite H. reflexivity.
 Qed.
 
 Lemma ann_R_pe_notOccur G G' s
 :  notOccur G' s
    -> G \ G' [=] G
    -> ann_R (@pe var _)
-           (ssa_ann s G)
-                     (mapAnn (pminus G') (ssa_ann s (G ∪ G'))).
+           (renamedApartAnn s G)
+                     (mapAnn (pminus G') (renamedApartAnn s (G ∪ G'))).
 Proof.
   intros. general induction H; simpl; try now (econstructor; reflexivity).
-  - assert ((G ++ G') ++ {x; {}} [=] (G ++ {{ x }}) ++ G'). {
+  - assert ({x ; G ++ G'} [=] {x; G} ++ G'). {
       cset_tac; intuition.
     }
     econstructor.
@@ -409,11 +143,9 @@ Proof.
       eapply H2 in H; intuition.
       rewrite <- H2.
       revert H; clear_all; cset_tac; intuition.
-      eapply H; cset_tac; eauto.
     + rewrite H3.
       eapply IHnotOccur.
       rewrite <- H2. revert H; clear_all; cset_tac; intuition.
-      eapply H. cset_tac; eauto.
   - econstructor; eauto.
     rewrite IHnotOccur1, IHnotOccur2; eauto.
     repeat rewrite getAnn_mapAnn.
@@ -421,10 +153,9 @@ Proof.
     repeat let_pair_case_eq; simpl; eauto.
     econstructor; try reflexivity.
     rewrite <- H2. clear_all; cset_tac; intuition.
-    rewrite minus_dist_union. reflexivity.
-  - econstructor. econstructor; rewrite <- H0; clear_all; cset_tac; intuition.
-  - econstructor. econstructor; rewrite <- H0; clear_all; cset_tac; intuition.
-  - assert ((G ++ G') ++ {x; {}} [=] (G ++ {{ x }}) ++ G'). {
+  - econstructor. econstructor. rewrite <- H0; cset_tac; intuition; eauto. reflexivity.
+  - econstructor. econstructor; try rewrite <- H0; clear_all; cset_tac; intuition.
+  - assert ({x ; G ++ G'} [=] {x; G} ++ G'). {
       cset_tac; intuition.
     }
     econstructor.
@@ -434,11 +165,9 @@ Proof.
       econstructor; try reflexivity.
       rewrite <- H2; clear_all; cset_tac; intuition.
       rewrite <- H2; revert H0; clear_all; cset_tac; intuition.
-      eapply H0; cset_tac; eauto.
     + rewrite H3.
       eapply IHnotOccur.
       rewrite <- H2; revert H0; clear_all; cset_tac; intuition.
-      eapply H0; cset_tac; eauto.
   - assert ((G ++ G') ++ of_list Z [=] (G ++ of_list Z) ++ G'). {
       cset_tac; intuition.
     }
@@ -448,9 +177,7 @@ Proof.
       let_pair_case_eq; simpl.
       econstructor. rewrite <- H2; clear_all; cset_tac; intuition.
       rewrite IHnotOccur2, getAnn_mapAnn.
-      unfold pminus. let_pair_case_eq; simpl.
-      rewrite minus_dist_union. reflexivity.
-      eauto.
+      unfold pminus. let_pair_case_eq; simpl; eauto. reflexivity. eauto.
       rewrite <- H2. revert H; clear_all; cset_tac; intuition; eauto.
     + rewrite H3.
       eapply IHnotOccur1.
@@ -458,219 +185,224 @@ Proof.
 Qed.
 
 
-Lemma rename_apart_ssa' (s:stmt) ϱ G
+Lemma freeVars_rename_exp_list ϱ Y
+  : list_union (List.map Exp.freeVars (List.map (rename_exp ϱ) Y))[=]
+               lookup_set ϱ (list_union (List.map Exp.freeVars Y)).
+Proof.
+  unfold list_union. rewrite lookup_set_list_union; eauto using lookup_set_empty.
+  repeat rewrite map_map. eapply fold_left_union_morphism; [|reflexivity].
+  clear_all. general induction Y; simpl; eauto using AllInRel.PIR2, freeVars_renameExp.
+Qed.
+
+Lemma freeVars_renamedApart' ϱ G s
+: lookup_set ϱ (freeVars s) ⊆ G
+  -> freeVars (snd (renameApart' ϱ G s)) [=] lookup_set ϱ (freeVars s).
+Proof.
+  general induction s; simpl; repeat let_pair_case_eq; simpl in * |- *; subst; eauto;
+          repeat rewrite lookup_set_union; try rewrite freeVars_renameExp; eauto; try reflexivity.
+  - rewrite IHs.
+    + rewrite lookup_set_update_union_minus; eauto.
+      assert (fresh G ∉ lookup_set ϱ (freeVars s \ {{x}})).
+      intro. eapply lookup_set_incl in H0; eauto.
+      eapply H in H0. eapply fresh_spec; eauto.
+      cset_tac; intuition.
+      cset_tac; intuition.
+    + rewrite lookup_set_update_in_union; eauto.
+      rewrite <- H at 3. repeat rewrite lookup_set_union; eauto.
+      cset_tac; intuition.
+  - rewrite IHs1, IHs2.
+    + reflexivity.
+    + rewrite <- H at 1. repeat rewrite lookup_set_union; eauto. cset_tac; intuition.
+    + rewrite <- H at 1. repeat rewrite lookup_set_union; eauto. cset_tac; intuition.
+  - eapply freeVars_rename_exp_list.
+  - rewrite IHs.
+    + rewrite freeVars_rename_exp_list.
+      rewrite lookup_set_update_union_minus; eauto.
+      assert (fresh G ∉ lookup_set ϱ (freeVars s \ {{x}})).
+      intro. eapply lookup_set_incl in H0; eauto.
+      eapply H in H0. eapply fresh_spec; eauto.
+      cset_tac; intuition.
+      cset_tac; intuition.
+    + rewrite lookup_set_update_in_union; eauto.
+      rewrite <- H at 3. repeat rewrite lookup_set_union; eauto.
+      cset_tac; intuition.
+  - rewrite IHs1, IHs2.
+    + rewrite lookup_set_update_union_minus_list; eauto.
+      rewrite lookup_set_union in H; eauto.
+      pose proof (fresh_list_spec _ fresh_spec G (length Z)).
+      cset_tac; intuition; eauto.
+      assert (a ∈ G). eapply H; eauto. cset_tac; intuition.
+      left; intuition; eauto.
+      rewrite fresh_list_length; eauto.
+    + rewrite <- H at 1. rewrite lookup_set_union; eauto.
+      cset_tac; intuition.
+    + rewrite lookup_set_update_with_list_in_union_length; eauto.
+      rewrite <- H at 2. rewrite lookup_set_union; eauto. cset_tac; intuition.
+      rewrite fresh_list_length; eauto.
+Qed.
+
+Lemma definedVars_renamedApart' ϱ G s
+: definedVars (snd (renameApart' ϱ G s)) [=] fst (renameApart' ϱ G s).
+Proof.
+  general induction s; simpl; repeat let_pair_case_eq; simpl in * |- *; subst; eauto;
+          repeat rewrite lookup_set_union; try rewrite freeVars_renameExp; eauto; try reflexivity.
+  - rewrite IHs; eauto; reflexivity.
+  - rewrite IHs1, IHs2; reflexivity.
+  - rewrite IHs; reflexivity.
+  - rewrite IHs1, IHs2. rewrite union_assoc. reflexivity.
+Qed.
+
+
+Lemma renameApart'_renamedApart (s:stmt) ϱ G
   : lookup_set ϱ (freeVars s) ⊆ G
-  -> ssa (snd (rename_apart' ϱ G s)) (ssa_ann (snd (rename_apart' ϱ G s)) G).
+  -> renamedApart (snd (renameApart' ϱ G s)) (renamedApartAnn (snd (renameApart' ϱ G s)) G).
 Proof.
   general induction s; simpl; repeat let_pair_case_eq; simpl.
-  - subst. econstructor; eauto using fresh_spec, ssa_ann_decomp.
+  - subst. econstructor; eauto using fresh_spec, renameApartAnn_decomp.
     + simpl in H.
       rewrite rename_exp_freeVars; eauto. etransitivity; eauto.
       eapply lookup_set_incl; eauto.
     + eapply IHs. simpl in *.
       hnf; intros. eapply lookup_set_spec in H0; eauto; dcr.
       lud.
-      * rewrite H3. cset_tac. right; eauto.
-      * rewrite union_comm. eapply incl_right. rewrite H3. eapply H.
+      * rewrite H3. cset_tac. left; eauto.
+      * cset_tac; intuition. right. rewrite H3. eapply H.
         eapply lookup_set_spec; eauto. eexists x0. split; eauto.
         eapply union_2. eapply in_in_minus; eauto. cset_tac; intuition.
+    + reflexivity.
   - subst s0 s4. simpl in H. simpl. rename s3 into Gs2. rename s into Gs1.
-    eapply ssaIf with (Ds := Gs1) (Dt := (Gs2 \ (Gs1 \ G))).
+    eapply renamedApartIf with (Ds := Gs1) (Dt := Gs2).
     + rewrite <- H. rewrite Exp.rename_exp_freeVars; eauto.
       eapply lookup_set_incl; eauto.
-    + eapply minus_incl_meet_special. subst; eapply rename_apart_incl. reflexivity.
-      subst. eapply rename_apart_incl; reflexivity.
-    + rewrite minus_incl_special. subst.
-      * rewrite <- ssa_ann_rename_apart.
-        rewrite ssa_ann_app_incl; try reflexivity.
-        rewrite <- ssa_ann_rename_apart.
-        rewrite ssa_ann_rename_apart.
-        rewrite rename_apart_fst_incl_app at 2. reflexivity.
-      * subst. eapply rename_apart_incl. reflexivity.
+    + assert (Gs1 ⊆ G ++ Gs1) by (cset_tac; intuition).
+      pose proof (renameApart'_disj ϱ (G ++ Gs1) s2).
+      rewrite H2, <- H0 in H3. eapply H3.
+    + repeat rewrite snd_renameApartAnn. subst; reflexivity.
     + subst. eapply IHs1. etransitivity; eauto. eapply lookup_set_incl; eauto.
-      eapply Subset_trans; [| eapply union_subset_1]. eapply union_subset_1.
-    + {
-        assert (G [=] (G \ (Gs1 \ G))) by eapply minus_minus_eq.
-        assert (Gs2 \ (Gs1 \ G) [=] (Gs2 \ (Gs1 \ G)) \ (Gs1 \ G))
-          by eapply minus_idem.
-        rewrite H0.
-        eapply ssa_minus. instantiate (1:=Gs1\G).
-        -  eapply notOccur_incl; try eapply rename_apart_notOccur with (G:=Gs1 \ G).
-          + eapply Subset_trans.
-            * rewrite minus_idem. reflexivity.
-            * eapply incl_minus_lr; try reflexivity.
-              eapply Subset_trans; eauto. eapply lookup_set_incl; eauto.
-              eapply Subset_trans; [| eapply union_subset_1]. eapply union_subset_2.
-          + eapply incl_minus.
-          + eapply Subset_trans.
-            * eapply Subset_trans; eauto. eapply lookup_set_incl; eauto.
-              eapply Subset_trans; [| eapply union_subset_1]. eapply union_subset_2.
-            * subst. eapply rename_apart_incl. reflexivity.
-        - eapply IHs2.
-          + eapply Subset_trans.
-            * eapply Subset_trans; eauto. eapply lookup_set_incl; eauto.
-              eapply Subset_trans; [| eapply union_subset_1]. eapply union_subset_2.
-            * subst. eapply rename_apart_incl. reflexivity.
-        -
-          intros. rewrite <- H0.
-          assert (G [=] (Gs1 \ (Gs1 \ G))). {
-          pose proof (@rename_apart_fst_incl ϱ s1 G). rewrite H1 in H4.
-          revert H4; clear_all; cset_tac; intuition.
-          decide (a ∈ G); eauto. exfalso. eauto.
-          }
-          assert (Gs1 [=] ((Gs1 \ (Gs1 \ G)) ++ (Gs1 \ G))). {
-          pose proof (@rename_apart_fst_incl ϱ s1 G). rewrite H1 in H5.
-          revert H4; clear_all; cset_tac; intuition.
-          decide (a ∈ G); intuition.
-          }
-          rewrite H4 at 1. rewrite H5 at 6. eapply ann_R_pe_notOccur.
-          eapply notOccur_incl; try eapply rename_apart_notOccur with (G:=Gs1 \ G).
-          + eapply Subset_trans.
-            * rewrite minus_idem. reflexivity.
-            * eapply incl_minus_lr; try reflexivity.
-              eapply Subset_trans; eauto. eapply lookup_set_incl; eauto.
-              eapply Subset_trans; [| eapply union_subset_1]. eapply union_subset_2.
-          + eapply incl_minus.
-          + eapply Subset_trans.
-            * eapply Subset_trans; eauto. eapply lookup_set_incl; eauto.
-              eapply Subset_trans; [| eapply union_subset_1]. eapply union_subset_2.
-            * subst. eapply rename_apart_incl. reflexivity.
-          + rewrite <- minus_idem. reflexivity.
+      cset_tac; intuition.
+    + pose proof (renameApart'_disj ϱ G s1). rewrite H1 in H0.
+      pose proof (renameApart'_disj ϱ (G ++ Gs1) s2). rewrite H2 in H3.
+      assert (notOccur Gs1 (snd (renameApart' ϱ (G ++ Gs1) s2))). {
+        eapply occurVars_disj_notOccur.
+        rewrite occurVars_freeVars_definedVars, disj_app.
+        rewrite freeVars_renamedApart'. split.
+        rewrite lookup_set_incl; eauto.
+        rewrite H. symmetry; eauto. cset_tac; intuition.
+        rewrite definedVars_renamedApart'. rewrite H2.
+        rewrite incl_right; eauto.
+        rewrite <- H. repeat rewrite lookup_set_union; cset_tac; intuition.
       }
-    + rewrite ssa_ann_decomp. rewrite ssa_ann_rename_apart.
+      eapply renamedApart_minus; [|eapply IHs2|eapply ann_R_pe_notOccur]; eauto.
+      * rewrite <- H. repeat rewrite lookup_set_union; cset_tac; intuition.
+      * eapply minus_inane_set, H0.
+    + rewrite renameApartAnn_decomp. rewrite snd_renameApartAnn.
       subst; reflexivity.
-    + rewrite ssa_ann_decomp. rewrite <- H2.
-      rewrite ssa_ann_rename_apart'. reflexivity.
-      subst. eapply rename_apart_fst_incl.
-
-  - econstructor. simpl in H.
+    + rewrite renameApartAnn_decomp. rewrite <- H2.
+      rewrite snd_renameApartAnn.
+      subst. reflexivity.
+  - econstructor; [| reflexivity]. simpl in H.
     rewrite <- H.
-    unfold list_union. rewrite lookup_set_list_union.
+    unfold list_union. rewrite lookup_set_list_union; eauto.
     instantiate (1:={}).
     eapply fold_left_subset_morphism; try reflexivity.
     repeat rewrite map_map.
     eapply map_ext_get; intros.
     rewrite <- Exp.rename_exp_freeVars; eauto; reflexivity.
-    hnf; intros. rewrite map_spec; eauto. cset_tac; intuition.
-    destruct H0; cset_tac; eauto. reflexivity.
+    eapply lookup_set_empty; eauto.
   - econstructor. simpl in H. rewrite <- H.
     rewrite Exp.rename_exp_freeVars; eauto.
     eapply lookup_set_incl; eauto.
     reflexivity. reflexivity.
-  - subst. econstructor; eauto using fresh_spec, ssa_ann_decomp.
+  - subst. econstructor; eauto using fresh_spec, renameApartAnn_decomp.
     + simpl in H.
       assert  (lookup_set ϱ
         (list_union (List.map Exp.freeVars Y)) [<=]G).
       rewrite <- H.
       eapply lookup_set_incl; eauto.
       rewrite <- H0.
-      unfold list_union. rewrite lookup_set_list_union.
+      unfold list_union. rewrite lookup_set_list_union; eauto.
       instantiate (1:={}).
       eapply fold_left_subset_morphism; try reflexivity.
       repeat rewrite map_map.
       eapply map_ext_get; intros.
       rewrite <- Exp.rename_exp_freeVars; eauto; reflexivity.
-      hnf; intros. rewrite map_spec; eauto. cset_tac; intuition.
-      destruct H1; cset_tac; eauto.
+      eapply lookup_set_empty; eauto.
     + eapply IHs. simpl in *.
       hnf; intros. eapply lookup_set_spec in H0; eauto; dcr.
       lud.
-      * rewrite H3. cset_tac. right; eauto.
-      * rewrite union_comm. eapply incl_right. rewrite H3. eapply H.
+      * rewrite H3. cset_tac. left; eauto.
+      * cset_tac. right. rewrite H3. eapply H.
         eapply lookup_set_spec; eauto. eexists x0. split; eauto.
         eapply union_2. eapply in_in_minus; eauto. cset_tac; intuition.
-
+    + reflexivity.
   - simpl. subst s0 s4. simpl in H. simpl. rename s3 into Gs2. rename s into Gs1.
-    eapply ssaLet with (Ds:=Gs1) (Dt:=Gs2 \ (Gs1 \ G)).
+    eapply renamedApartLet with (Ds:=Gs1) (Dt:=Gs2).
     + eapply fresh_set_spec. eapply fresh_spec.
-    + eapply  minus_incl_meet_special; eauto using rename_apart_incl_eq, incl_refl.
-      subst. eapply rename_apart_incl. eapply incl_left.
-      subst. eapply rename_apart_incl. eapply Subset_refl.
-    + rewrite ssa_ann_rename_apart; try reflexivity.
+    + pose proof (renameApart'_disj ϱ (G ++ (Gs1 ++ of_list (fresh_list fresh G (length Z)))) s2).
+      rewrite H2 in H0.
+      pose proof (renameApart'_disj (ϱ [Z <-- fresh_list fresh G (length Z)])
+                                    (G ++ of_list (fresh_list fresh G (length Z))) s1).
+      rewrite H1 in H3.
+      revert H0 H3; unfold disj; clear_all; cset_tac; intuition; eauto.
+    + rewrite snd_renameApartAnn; try reflexivity.
       rewrite H1.
-      rewrite ssa_ann_rename_apart'. rewrite H2. reflexivity.
-      subst Gs1.
-      rewrite <- rename_apart_fst_incl. eapply incl_left.
+      rewrite snd_renameApartAnn; try reflexivity.
+      rewrite H2. cset_tac; intuition.
     + eapply IHs1.
       rewrite lookup_set_update_with_list_in_union_length; eauto.
       eapply incl_union_lr; eauto. rewrite <- H.
       eapply lookup_set_incl; eauto. intuition. reflexivity.
       rewrite fresh_list_length; eauto.
-    + rewrite ssa_ann_decomp.
+    + rewrite renameApartAnn_decomp.
       econstructor. rewrite union_comm. reflexivity.
-      rewrite ssa_ann_rename_apart. subst; reflexivity.
-    +  {
-        assert (G [=] (G \ (Gs1 \ G))) by eapply minus_minus_eq.
-        assert (Gs2 \ (Gs1 \ G) [=] (Gs2 \ (Gs1 \ G)) \ (Gs1 \ G))
-          by eapply minus_idem.
-        rewrite H0.
-        eapply ssa_minus. instantiate (1:=Gs1\G).
-        -  eapply notOccur_incl; try eapply rename_apart_notOccur with (G:=Gs1 \ G).
-          + eapply Subset_trans.
-            * rewrite minus_idem. reflexivity.
-            * eapply incl_minus_lr; try reflexivity.
-              eapply Subset_trans; eauto. eapply lookup_set_incl; eauto.
-          + eapply incl_minus.
-          + eapply Subset_trans.
-            * eapply Subset_trans; eauto. eapply lookup_set_incl; eauto.
-            * subst. eapply rename_apart_incl. eapply incl_left.
-        - eapply IHs2.
-          + eapply Subset_trans.
-            * eapply Subset_trans; eauto. eapply lookup_set_incl; eauto.
-            * subst. eapply rename_apart_incl. eapply incl_left.
-        -
-          intros. rewrite <- H0.
-          assert (G [=] (Gs1 \ (Gs1 \ G))). {
-            assert (G ⊆ Gs1). rewrite <- H1.
-            rewrite <- rename_apart_fst_incl. eapply incl_left.
-            revert H4; clear_all; cset_tac; intuition.
-            decide (a ∈ G); eauto. exfalso. eauto.
-          }
-          assert (Gs1 [=] ((Gs1 \ (Gs1 \ G)) ++ (Gs1 \ G))). {
-            assert (G ⊆ Gs1). rewrite <- H1.
-            rewrite <- rename_apart_fst_incl. eapply incl_left.
-            revert H5; clear_all; cset_tac; intuition.
-            decide (a ∈ G); intuition.
-          }
-          rewrite H4 at 1. rewrite H5 at 6. eapply ann_R_pe_notOccur.
-          eapply notOccur_incl; try eapply rename_apart_notOccur with (G:=Gs1 \ G).
-          + eapply Subset_trans.
-            * rewrite minus_idem. reflexivity.
-            * eapply incl_minus_lr; try reflexivity.
-              eapply Subset_trans; eauto. eapply lookup_set_incl; eauto.
-          + eapply incl_minus.
-          + eapply Subset_trans.
-            * eapply Subset_trans; eauto. eapply lookup_set_incl; eauto.
-            * subst. eapply rename_apart_incl. eapply incl_left.
-          + rewrite <- minus_idem. reflexivity.
+      rewrite snd_renameApartAnn. subst; reflexivity.
+    + pose proof (renameApart'_disj (ϱ [Z <-- fresh_list fresh G (length Z)])
+                                    (G ++ of_list (fresh_list fresh G (length Z))) s1).
+      rewrite H1 in H0.
+      pose proof (renameApart'_disj ϱ (G ++ Gs1 ++ of_list (fresh_list fresh G (length Z))) s2).
+      rewrite H2 in H3.
+      assert (notOccur (Gs1 ++ of_list (fresh_list fresh G (length Z))) (snd (renameApart' ϱ (G ++ Gs1 ++ of_list (fresh_list fresh G (length Z))) s2))). {
+        eapply occurVars_disj_notOccur.
+        rewrite occurVars_freeVars_definedVars, disj_app.
+        rewrite freeVars_renamedApart'. split.
+        rewrite lookup_set_incl; eauto.
+        rewrite H. symmetry. rewrite disj_app; split.
+        rewrite incl_left; eauto.
+        symmetry; eapply fresh_list_spec, fresh_spec.
+        cset_tac; intuition.
+        rewrite definedVars_renamedApart'. rewrite H2.
+        rewrite incl_right; eauto.
+        rewrite <- H at 1. repeat rewrite lookup_set_union; cset_tac; intuition.
       }
-    + rewrite ssa_ann_decomp. econstructor. reflexivity.
-      rewrite ssa_ann_rename_apart'. rewrite H2. reflexivity.
-      rewrite <- H1. rewrite <- rename_apart_fst_incl.
-      eapply incl_left.
+      eapply renamedApart_minus; [|eapply IHs2| eapply ann_R_pe_notOccur]; eauto.
+      * rewrite <- H at 1. rewrite lookup_set_union; cset_tac; intuition.
+      * eapply minus_inane_set. change (disj G (Gs1 ++ of_list (fresh_list fresh G (length Z)))).
+        eapply disj_app. split.
+        rewrite incl_left; eauto.
+        symmetry. eapply fresh_list_spec, fresh_spec.
+    + rewrite renameApartAnn_decomp. econstructor. reflexivity.
+      rewrite snd_renameApartAnn. rewrite H2. reflexivity.
     + eapply fresh_list_unique. eapply fresh_spec.
 Qed.
 
 Lemma rename_apart_alpha' G ϱ ϱ' s
   : lookup_set ϱ (freeVars s) ⊆ G
   -> inverse_on (freeVars s) ϱ ϱ'
-  -> alpha ϱ' ϱ (snd (rename_apart' ϱ G s)) s.
+  -> alpha ϱ' ϱ (snd (renameApart' ϱ G s)) s.
 Proof.
   general induction s; simpl; repeat let_pair_case_eq; subst; simpl in * |- *; eauto using alpha.
 
   - econstructor. eapply alpha_exp_sym. eapply alpha_exp_rename_injective.
     eapply inverse_on_incl; eauto. cset_tac; eauto.
     eapply IHs.
-    + rewrite lookup_set_update_in_union.
-      eapply incl_union_lr; try reflexivity. rewrite <- H.
-      eapply lookup_set_incl. intuition. cset_tac; eauto. intuition.
+    + rewrite <- H at 3. rewrite lookup_set_update_in_union; intuition.
+      rewrite lookup_set_union; cset_tac; intuition.
     + eapply inverse_on_update_inverse. intuition.
       eapply inverse_on_incl; eauto. cset_tac; eauto.
       assert (lookup_set ϱ (freeVars s \ {{x}}) ⊆
                          lookup_set ϱ (freeVars s \ {{x}} ∪ Exp.freeVars e)).
-      eapply lookup_set_incl. intuition. cset_tac; eauto.
-      intro. eapply H1 in H2. eapply H in H2.
-      eapply fresh_spec in H2. eauto.
+      rewrite lookup_set_union; cset_tac; intuition.
+      rewrite H1, H. eapply fresh_spec; eauto.
   - econstructor; eauto.
     + eapply alpha_exp_sym. eapply Exp.alpha_exp_rename_injective.
       eapply inverse_on_incl; eauto. eapply incl_right.
@@ -679,10 +411,9 @@ Proof.
         rewrite union_assoc, union_comm. eapply incl_right.
       * eapply inverse_on_incl; eauto. rewrite union_assoc, union_comm. eapply incl_right.
     + eapply IHs2; eauto.
-      * eapply Subset_trans; eauto using rename_apart_incl. eapply lookup_set_incl; [intuition|].
-        rewrite union_comm at 1. rewrite <- union_assoc. eapply incl_right.
+      * rewrite <- H at 1. repeat rewrite lookup_set_union; cset_tac; intuition.
       * eapply inverse_on_incl; eauto.
-        rewrite union_comm at 1. rewrite <- union_assoc. eapply incl_right.
+        cset_tac; intuition.
   - econstructor. rewrite map_length; eauto.
     intros. edestruct map_get_4; eauto; dcr; get_functional; subst.
     eapply alpha_exp_sym. eapply Exp.alpha_exp_rename_injective.
@@ -701,14 +432,14 @@ Proof.
       eapply  incl_list_union; try reflexivity.
       eapply map_get_1; eauto.
     + eapply IHs; eauto.
-      * rewrite lookup_set_update_in_union.
-        eapply incl_union_lr; try reflexivity. rewrite <- H.
-        eapply lookup_set_incl. intuition. cset_tac; eauto. intuition.
+      * rewrite <- H at 3. rewrite lookup_set_update_in_union; intuition.
+        rewrite lookup_set_union; cset_tac; intuition.
       * eapply inverse_on_update_inverse. intuition.
         eapply inverse_on_incl; eauto. cset_tac; eauto.
-        rewrite lookup_set_incl; [ | eauto | eapply incl_left; eauto].
-        erewrite H.
-        eapply fresh_spec.
+        assert (lookup_set ϱ (freeVars s \ {{x}}) ⊆
+                           lookup_set ϱ (freeVars s \ {{x}} ∪ list_union (List.map Exp.freeVars Y))).
+        rewrite lookup_set_union; cset_tac; intuition.
+        rewrite H1, H. eapply fresh_spec; eauto.
   - econstructor. eapply fresh_list_length.
     + eapply IHs1.
       * rewrite lookup_set_update_with_list_in_union_length.
@@ -719,27 +450,24 @@ Proof.
         eapply inverse_on_incl; eauto; cset_tac; eauto.
         eapply fresh_list_unique. eapply fresh_spec.
         rewrite fresh_list_length; eauto.
-        hnf; intros. intro. eapply lookup_set_spec in H2.
-        destruct H2; dcr; cset_tac.
-        pose proof (fresh_list_spec fresh fresh_spec G (length Z)).
-        assert (x ∈ G). rewrite <- H.
-        eapply lookup_set_spec. intuition.
-        eexists x0. cset_tac; intuition.
-        eapply (not_in_empty x).
-        eapply fresh_list_spec. eapply fresh_spec. cset_tac; eauto. intuition.
+        assert (lookup_set ϱ (freeVars s1 \ of_list Z) ⊆
+                           lookup_set ϱ ((freeVars s1 \ of_list Z) ++ freeVars s2)).
+        rewrite lookup_set_union; cset_tac; intuition.
+        rewrite H1. rewrite H. eapply fresh_list_spec, fresh_spec.
     + eapply IHs2.
-      * eapply rename_apart_incl. eapply Subset_trans; [| eapply  union_subset_1].
-        eapply Subset_trans; eauto. eapply lookup_set_incl;[intuition| eapply incl_right].
+      * rewrite <- H at 1.
+        rewrite lookup_set_union; eauto. cset_tac; intuition.
       * eapply inverse_on_incl; eauto. eapply incl_right.
 Qed.
 
 (** Based on [rename_apart'], we can define a function that renames apart bound variables apart
     and keeps free variables the same *)
-Definition rename_apart s := snd (rename_apart' id (freeVars s) s).
+Definition rename_apart s := snd (renameApart' id (freeVars s) s).
 
-Lemma rename_apart_ssa (s:stmt)
-  : ssa (rename_apart s) (ssa_ann (snd (rename_apart' id (freeVars s) s)) (freeVars s)).
-  eapply rename_apart_ssa'. eapply lookup_set_on_id. reflexivity.
+Lemma rename_apart_renamedApart (s:stmt)
+: renamedApart (rename_apart s)
+               (renamedApartAnn (snd (renameApart' id (freeVars s) s)) (freeVars s)).
+  eapply renameApart'_renamedApart. eapply lookup_set_on_id. reflexivity.
 Qed.
 
 Lemma rename_apart_alpha s
