Constr/MapLookup.v
@@ -121,6 +121,20 @@ Proof.
   eapply lookup_set_spec; eauto.
 Qed.
 
+Lemma lookup_set_add X `{OrderedType X} Y `{OrderedType Y} x s (m:X -> Y) `{Proper _ (_eq ==> _eq) m}
+: (lookup_set m {x; s}) [=] {m x; lookup_set m s}.
+Proof.
+  intro. split; intros.
+  - eapply lookup_set_spec in H2; eauto.
+    cset_tac. destruct H4.
+    + left; rewrite H2; symmetry; eauto.
+    + right; eapply lookup_set_spec; firstorder.
+  - cset_tac. destruct H2; eapply lookup_set_spec; dcr; eauto.
+    + eexists x; cset_tac; firstorder.
+    + eapply lookup_set_spec in H2; eauto.
+      firstorder.
+Qed.
+
 Ltac set_tac :=
   repeat cset_tac;
   match goal with
@@ -129,6 +143,22 @@ Ltac set_tac :=
     | [ |- context [ In ?y (lookup_set ?f ?s) ]] =>
       rewrite (@lookup_set_spec _ _ _ _ f s y)
   end.
+
+
+Lemma lookup_set_empty X `{OrderedType X} Y `{OrderedType Y} (ϱ:X->Y)
+      `{Proper _ (_eq ==> _eq) ϱ}
+: lookup_set ϱ {} [=] {}.
+Proof.
+  unfold lookup_set. cset_tac.
+  rewrite map_iff; eauto.
+  firstorder. cset_tac; eauto.
+Qed.
+
+Hint Extern 20 (lookup_set ?ϱ {} [=] {}) => eapply lookup_set_empty; eauto.
+Hint Extern 20 ({} [=] lookup_set ?ϱ {}) => symmetry; eapply lookup_set_empty; eauto.
+
+Hint Extern 20 (lookup_set ?ϱ (singleton ?v) [=] singleton (?ϱ ?v)) => eapply lookup_set_singleton'; eauto.
+Hint Extern 20 (singleton (?ϱ ?v) [=] lookup_set ?ϱ (singleton ?v)) => symmetry; eapply lookup_set_singleton'; eauto.
 
 (*
  *** Local Variables: ***
